<?xml version="1.0"?>
<rdf:RDF xmlns="http://www.semanticweb.org/sten-doipanni/ontologies/2021/3/exuvia.owl#"
     xml:base="http://www.semanticweb.org/sten-doipanni/ontologies/2021/3/exuvia.owl"
     xmlns:ex="http://www.semanticweb.org/sten-doipanni/ontologies/2021/3/exuvia.owl#"
     xmlns:owl="http://www.w3.org/2002/07/owl#"
     xmlns:rdf="http://www.w3.org/1999/02/22-rdf-syntax-ns#"
     xmlns:xml="http://www.w3.org/XML/1998/namespace"
     xmlns:xsd="http://www.w3.org/2001/XMLSchema#"
     xmlns:opla="http://ontologydesignpatterns.org/opla#"
     xmlns:rdfs="http://www.w3.org/2000/01/rdf-schema#">
    <owl:Ontology rdf:about="http://www.semanticweb.org/sten-doipanni/ontologies/2021/3/exuvia.owl">
        <rdfs:comment>Exuviae is the intensional epistemological vocabulary elaborated for the COntPare methodology.
It is developed to allow basic epistemic operations in theory comparison: conceptual derivations, components clustering and components selection

Version 1.0 : 29.04.2021

Designed by Stefano De Giorgis and Aldo Gangemi.</rdfs:comment>
    </owl:Ontology>
    


    <!-- 
    ///////////////////////////////////////////////////////////////////////////////////////
    //
    // Annotation properties
    //
    ///////////////////////////////////////////////////////////////////////////////////////
     -->

    


    <!-- http://www.semanticweb.org/sten-doipanni/ontologies/2021/3/exuvia.owl#bibRef -->

    <owl:AnnotationProperty rdf:about="http://www.semanticweb.org/sten-doipanni/ontologies/2021/3/exuvia.owl#bibRef"/>
    


    <!-- 
    ///////////////////////////////////////////////////////////////////////////////////////
    //
    // Object Properties
    //
    ///////////////////////////////////////////////////////////////////////////////////////
     -->

    


    <!-- http://www.semanticweb.org/sten-doipanni/ontologies/2021/3/exuvia.owl#conceptuallyDerivedFrom -->

    <owl:ObjectProperty rdf:about="http://www.semanticweb.org/sten-doipanni/ontologies/2021/3/exuvia.owl#conceptuallyDerivedFrom">
        <owl:inverseOf rdf:resource="http://www.semanticweb.org/sten-doipanni/ontologies/2021/3/exuvia.owl#isConceptualSourceFor"/>
        <rdf:type rdf:resource="http://www.w3.org/2002/07/owl#TransitiveProperty"/>
        <rdfs:domain>
            <owl:Class>
                <owl:unionOf rdf:parseType="Collection">
                    <rdf:Description rdf:about="http://www.ontologydesignpatterns.org/ont/dul/DUL.owl#Theory"/>
                    <rdf:Description rdf:about="http://www.semanticweb.org/sten-doipanni/ontologies/2021/3/exuvia.owl#TheoreticalFragment"/>
                </owl:unionOf>
            </owl:Class>
        </rdfs:domain>
        <rdfs:comment>An entity conceptuallyDerivedFrom some other entity has an intellectual debt to the latter, meaning that in some way, the former entity e.g. a dul:Concept was elaborated starting from some clue, intuition, concept, rule or theory that gave the input in a more or less decisevely way to a Cognizer for its cognition of the Concept.
Note that also the way in which some Entity is derived from some other Entity could be the the object of a conceptual derivation, and if different conceptual derivation are competing the subproperties could be used to clarify the nuances.</rdfs:comment>
    </owl:ObjectProperty>
    


    <!-- http://www.semanticweb.org/sten-doipanni/ontologies/2021/3/exuvia.owl#contradicts -->

    <owl:ObjectProperty rdf:about="http://www.semanticweb.org/sten-doipanni/ontologies/2021/3/exuvia.owl#contradicts">
        <rdfs:subPropertyOf rdf:resource="http://www.semanticweb.org/sten-doipanni/ontologies/2021/3/exuvia.owl#conceptuallyDerivedFrom"/>
        <owl:inverseOf rdf:resource="http://www.semanticweb.org/sten-doipanni/ontologies/2021/3/exuvia.owl#isContradictedBy"/>
        <rdfs:comment>Some Entity or part of it is derived and then contradicted or negated, totally or partially.</rdfs:comment>
    </owl:ObjectProperty>
    


    <!-- http://www.semanticweb.org/sten-doipanni/ontologies/2021/3/exuvia.owl#explicates -->

    <owl:ObjectProperty rdf:about="http://www.semanticweb.org/sten-doipanni/ontologies/2021/3/exuvia.owl#explicates">
        <rdfs:subPropertyOf rdf:resource="http://www.semanticweb.org/sten-doipanni/ontologies/2021/3/exuvia.owl#reframes"/>
        <owl:inverseOf rdf:resource="http://www.semanticweb.org/sten-doipanni/ontologies/2021/3/exuvia.owl#isExplicatedBy"/>
        <rdfs:comment>A way to express some logical or formal conclusion explicitly declared by the conceptually derived entity and implied, but not declared explicitly by the source.</rdfs:comment>
    </owl:ObjectProperty>
    


    <!-- http://www.semanticweb.org/sten-doipanni/ontologies/2021/3/exuvia.owl#generalizes -->

    <owl:ObjectProperty rdf:about="http://www.semanticweb.org/sten-doipanni/ontologies/2021/3/exuvia.owl#generalizes">
        <rdfs:subPropertyOf rdf:resource="http://www.semanticweb.org/sten-doipanni/ontologies/2021/3/exuvia.owl#conceptuallyDerivedFrom"/>
        <owl:inverseOf rdf:resource="http://www.semanticweb.org/sten-doipanni/ontologies/2021/3/exuvia.owl#isGeneralizedBy"/>
        <rdfs:comment>The derived entity corresponds to a broader extension than
the source, this poperty is similar to the skos:broadMatch property, but referred to conceptual objects.</rdfs:comment>
    </owl:ObjectProperty>
    


    <!-- http://www.semanticweb.org/sten-doipanni/ontologies/2021/3/exuvia.owl#hasCriterionMeasurement -->

    <owl:ObjectProperty rdf:about="http://www.semanticweb.org/sten-doipanni/ontologies/2021/3/exuvia.owl#hasCriterionMeasurement">
        <rdfs:domain rdf:resource="http://www.semanticweb.org/sten-doipanni/ontologies/2021/3/exuvia.owl#SelectionCriterion"/>
        <rdfs:range rdf:resource="http://www.semanticweb.org/sten-doipanni/ontologies/2021/3/exuvia.owl#CriterionMeasurement"/>
    </owl:ObjectProperty>
    


    <!-- http://www.semanticweb.org/sten-doipanni/ontologies/2021/3/exuvia.owl#hasReframingModus -->

    <owl:ObjectProperty rdf:about="http://www.semanticweb.org/sten-doipanni/ontologies/2021/3/exuvia.owl#hasReframingModus">
        <rdfs:subPropertyOf rdf:resource="http://www.w3.org/2002/07/owl#topObjectProperty"/>
        <rdfs:range rdf:resource="http://www.semanticweb.org/sten-doipanni/ontologies/2021/3/exuvia.owl#ReframingModus"/>
        <rdfs:comment>The &quot;modus&quot; in which some Entity reframes some other entity. It could be the perspective, the contextual considered knowledge, the interpretation etc.</rdfs:comment>
    </owl:ObjectProperty>
    


    <!-- http://www.semanticweb.org/sten-doipanni/ontologies/2021/3/exuvia.owl#hasSelectionCriterion -->

    <owl:ObjectProperty rdf:about="http://www.semanticweb.org/sten-doipanni/ontologies/2021/3/exuvia.owl#hasSelectionCriterion">
        <rdfs:range rdf:resource="http://www.semanticweb.org/sten-doipanni/ontologies/2021/3/exuvia.owl#SelectionCriterion"/>
    </owl:ObjectProperty>
    


    <!-- http://www.semanticweb.org/sten-doipanni/ontologies/2021/3/exuvia.owl#isConceptualSourceFor -->

    <owl:ObjectProperty rdf:about="http://www.semanticweb.org/sten-doipanni/ontologies/2021/3/exuvia.owl#isConceptualSourceFor">
        <rdfs:domain>
            <owl:Class>
                <owl:unionOf rdf:parseType="Collection">
                    <rdf:Description rdf:about="http://www.ontologydesignpatterns.org/ont/dul/DUL.owl#Theory"/>
                    <rdf:Description rdf:about="http://www.semanticweb.org/sten-doipanni/ontologies/2021/3/exuvia.owl#TheoreticalFragment"/>
                </owl:unionOf>
            </owl:Class>
        </rdfs:domain>
    </owl:ObjectProperty>
    


    <!-- http://www.semanticweb.org/sten-doipanni/ontologies/2021/3/exuvia.owl#isContradictedBy -->

    <owl:ObjectProperty rdf:about="http://www.semanticweb.org/sten-doipanni/ontologies/2021/3/exuvia.owl#isContradictedBy">
        <rdfs:subPropertyOf rdf:resource="http://www.semanticweb.org/sten-doipanni/ontologies/2021/3/exuvia.owl#isConceptualSourceFor"/>
    </owl:ObjectProperty>
    


    <!-- http://www.semanticweb.org/sten-doipanni/ontologies/2021/3/exuvia.owl#isExplicatedBy -->

    <owl:ObjectProperty rdf:about="http://www.semanticweb.org/sten-doipanni/ontologies/2021/3/exuvia.owl#isExplicatedBy">
        <rdfs:subPropertyOf rdf:resource="http://www.semanticweb.org/sten-doipanni/ontologies/2021/3/exuvia.owl#isConceptualSourceFor"/>
    </owl:ObjectProperty>
    


    <!-- http://www.semanticweb.org/sten-doipanni/ontologies/2021/3/exuvia.owl#isGeneralizedBy -->

    <owl:ObjectProperty rdf:about="http://www.semanticweb.org/sten-doipanni/ontologies/2021/3/exuvia.owl#isGeneralizedBy">
        <rdfs:subPropertyOf rdf:resource="http://www.semanticweb.org/sten-doipanni/ontologies/2021/3/exuvia.owl#isConceptualSourceFor"/>
    </owl:ObjectProperty>
    


    <!-- http://www.semanticweb.org/sten-doipanni/ontologies/2021/3/exuvia.owl#isReframedBy -->

    <owl:ObjectProperty rdf:about="http://www.semanticweb.org/sten-doipanni/ontologies/2021/3/exuvia.owl#isReframedBy">
        <rdfs:subPropertyOf rdf:resource="http://www.semanticweb.org/sten-doipanni/ontologies/2021/3/exuvia.owl#isConceptualSourceFor"/>
        <owl:inverseOf rdf:resource="http://www.semanticweb.org/sten-doipanni/ontologies/2021/3/exuvia.owl#reframes"/>
    </owl:ObjectProperty>
    


    <!-- http://www.semanticweb.org/sten-doipanni/ontologies/2021/3/exuvia.owl#isSpecifiedBy -->

    <owl:ObjectProperty rdf:about="http://www.semanticweb.org/sten-doipanni/ontologies/2021/3/exuvia.owl#isSpecifiedBy">
        <rdfs:subPropertyOf rdf:resource="http://www.semanticweb.org/sten-doipanni/ontologies/2021/3/exuvia.owl#isConceptualSourceFor"/>
        <owl:inverseOf rdf:resource="http://www.semanticweb.org/sten-doipanni/ontologies/2021/3/exuvia.owl#specifies"/>
    </owl:ObjectProperty>
    


    <!-- http://www.semanticweb.org/sten-doipanni/ontologies/2021/3/exuvia.owl#reframes -->

    <owl:ObjectProperty rdf:about="http://www.semanticweb.org/sten-doipanni/ontologies/2021/3/exuvia.owl#reframes">
        <rdfs:subPropertyOf rdf:resource="http://www.semanticweb.org/sten-doipanni/ontologies/2021/3/exuvia.owl#conceptuallyDerivedFrom"/>
        <rdfs:comment>The derived entity is in some way changed during the derivation,
it is highly recommended to specify what components of an entity are reframed and in which way.</rdfs:comment>
    </owl:ObjectProperty>
    


    <!-- http://www.semanticweb.org/sten-doipanni/ontologies/2021/3/exuvia.owl#reuses -->

    <owl:ObjectProperty rdf:about="http://www.semanticweb.org/sten-doipanni/ontologies/2021/3/exuvia.owl#reuses">
        <rdfs:subPropertyOf rdf:resource="http://www.semanticweb.org/sten-doipanni/ontologies/2021/3/exuvia.owl#conceptuallyDerivedFrom"/>
        <rdf:type rdf:resource="http://www.w3.org/2002/07/owl#TransitiveProperty"/>
        <rdfs:comment>The derived entity is copied and reused (cloned), with possible minimal and not substantial nuanced distinctions e.g. re-labeling without new semantic commitment.</rdfs:comment>
    </owl:ObjectProperty>
    


    <!-- http://www.semanticweb.org/sten-doipanni/ontologies/2021/3/exuvia.owl#specifies -->

    <owl:ObjectProperty rdf:about="http://www.semanticweb.org/sten-doipanni/ontologies/2021/3/exuvia.owl#specifies">
        <rdfs:subPropertyOf rdf:resource="http://www.semanticweb.org/sten-doipanni/ontologies/2021/3/exuvia.owl#conceptuallyDerivedFrom"/>
        <rdfs:comment>The derived entity specializes in some way the source, this property is
also aligned to dul:specializes.</rdfs:comment>
    </owl:ObjectProperty>
    


    <!-- 
    ///////////////////////////////////////////////////////////////////////////////////////
    //
    // Classes
    //
    ///////////////////////////////////////////////////////////////////////////////////////
     -->

    


    <!-- http://www.ontologydesignpatterns.org/ont/dul/DUL.owl#Theory -->

    <owl:Class rdf:about="http://www.ontologydesignpatterns.org/ont/dul/DUL.owl#Theory"/>
    


    <!-- http://www.semanticweb.org/sten-doipanni/ontologies/2021/3/exuvia.owl#CriterionMeasurement -->

    <owl:Class rdf:about="http://www.semanticweb.org/sten-doipanni/ontologies/2021/3/exuvia.owl#CriterionMeasurement">
        <rdfs:comment>The Measurement of the Criterion chosen to select a Fragment against another. e.g. better literature grounding, more soundness, better resources at disposal, more operationalizable structure etc.</rdfs:comment>
    </owl:Class>
    


    <!-- http://www.semanticweb.org/sten-doipanni/ontologies/2021/3/exuvia.owl#ReframingModus -->

    <owl:Class rdf:about="http://www.semanticweb.org/sten-doipanni/ontologies/2021/3/exuvia.owl#ReframingModus">
        <rdfs:comment>The &quot;modus&quot; in which some Entity reframes some other entity. It could be the perspective, the contextual considered knowledge, the interpretation etc.</rdfs:comment>
    </owl:Class>
    


    <!-- http://www.semanticweb.org/sten-doipanni/ontologies/2021/3/exuvia.owl#SelectionCriterion -->

    <owl:Class rdf:about="http://www.semanticweb.org/sten-doipanni/ontologies/2021/3/exuvia.owl#SelectionCriterion">
        <rdfs:comment>The Criterion based on which some Selection is made.
e.g. in a Debate Competition in order to support some topic some pieces of information are selected as argument based on some criterion. The criterion could be e.g. the soundness of the argument, the popularity of the topic, the scientific evidence supporting it etc.</rdfs:comment>
    </owl:Class>
    


    <!-- http://www.semanticweb.org/sten-doipanni/ontologies/2021/3/exuvia.owl#TheoreticalFragment -->

    <owl:Class rdf:about="http://www.semanticweb.org/sten-doipanni/ontologies/2021/3/exuvia.owl#TheoreticalFragment">
        <rdfs:comment>A TheoreticalFragment is a theoretical object, a sort of semantic field which contains things related in some way one with the others. 
The semantic field derives from manual comparing of different theories. Behind the idea of fragment there is a particular epistemology, that is the choice epistemology for which there are different choices possible and a final one made based on some criterion and the measurement of the selected criterion.</rdfs:comment>
    </owl:Class>
    


    <!-- http://www.semanticweb.org/sten-doipanni/ontologies/2021/3/exuvia.owl#TheorySelectionFrame -->

    <owl:Class rdf:about="http://www.semanticweb.org/sten-doipanni/ontologies/2021/3/exuvia.owl#TheorySelectionFrame">
        <rdfs:comment>The frame in which some TheoryFragment is selected to be introduced in a Theory. The frame takes as roles:
- TheoreticalFragment as the Entity isolated to be compared.
- SelectionCriterion as the criterion on which the selection could happen.
- CriterionMeasurement as the measurement of the selected criterion.</rdfs:comment>
    </owl:Class>
</rdf:RDF>



<!-- Generated by the OWL API (version 4.5.9.2019-02-01T07:24:44Z) https://github.com/owlcs/owlapi -->

