<?xml version="1.0"?>
<rdf:RDF xmlns="http://www.ontologydesignpatterns.org/ont/is/mandlerpaganis.owl#"
     xml:base="http://www.ontologydesignpatterns.org/ont/is/mandlerpaganis.owl"
     xmlns:owl="http://www.w3.org/2002/07/owl#"
     xmlns:rdf="http://www.w3.org/1999/02/22-rdf-syntax-ns#"
     xmlns:xml="http://www.w3.org/XML/1998/namespace"
     xmlns:xsd="http://www.w3.org/2001/XMLSchema#"
     xmlns:opla="http://ontologydesignpatterns.org/opla#"
     xmlns:rdfs="http://www.w3.org/2000/01/rdf-schema#"
     xmlns:ismeta="http://www.ontologydesignpatterns.org/ont/is/ismeta.owl#"
     xmlns:mandlerpaganis="http://www.ontologydesignpatterns.org/ont/is/mandlerpaganis.owl#">
    <owl:Ontology rdf:about="http://www.ontologydesignpatterns.org/ont/is/mandlerpaganis.owl">
        <rdfs:comment>Ontological version of Mandler &amp; Pagán Cánovas theory about Image Schemas and Spatial Primitives, with a particular focus on Developmental Perspective psychology approach.
 
MPC module of ISAAC ontology: an ontology for Image Schemas Analysis And Comparison.

Designed by Stefano De Giorgis and Aldo Gangemi.</rdfs:comment>
    </owl:Ontology>
    


    <!-- 
    ///////////////////////////////////////////////////////////////////////////////////////
    //
    // Annotation properties
    //
    ///////////////////////////////////////////////////////////////////////////////////////
     -->

    


    <!-- http://www.ontologydesignpatterns.org/ont/is/ismeta.owl#bibRef -->

    <owl:AnnotationProperty rdf:about="http://www.ontologydesignpatterns.org/ont/is/ismeta.owl#bibRef"/>
    


    <!-- 
    ///////////////////////////////////////////////////////////////////////////////////////
    //
    // Object Properties
    //
    ///////////////////////////////////////////////////////////////////////////////////////
     -->

    


    <!-- http://www.ontologydesignpatterns.org/ont/is/mandlerpaganis.owl#combinationResultsFrom -->

    <owl:ObjectProperty rdf:about="http://www.ontologydesignpatterns.org/ont/is/mandlerpaganis.owl#combinationResultsFrom">
        <rdfs:domain rdf:resource="http://www.ontologydesignpatterns.org/ont/is/mandlerpaganis.owl#IS_Combination"/>
        <rdfs:range>
            <owl:Class>
                <owl:unionOf rdf:parseType="Collection">
                    <rdf:Description rdf:about="http://www.ontologydesignpatterns.org/ont/is/mandlerpaganis.owl#ImageSchema"/>
                    <rdf:Description rdf:about="http://www.ontologydesignpatterns.org/ont/is/mandlerpaganis.owl#SpatialPrimitive"/>
                </owl:unionOf>
            </owl:Class>
        </rdfs:range>
        <rdfs:comment>Some IS_Combination is the combinationResult of some ImageSchema and/or SpatialPrimitive that combines together.</rdfs:comment>
    </owl:ObjectProperty>
    


    <!-- http://www.ontologydesignpatterns.org/ont/is/mandlerpaganis.owl#groupedIn -->

    <owl:ObjectProperty rdf:about="http://www.ontologydesignpatterns.org/ont/is/mandlerpaganis.owl#groupedIn">
        <owl:inverseOf rdf:resource="http://www.ontologydesignpatterns.org/ont/is/mandlerpaganis.owl#groups"/>
        <rdfs:domain>
            <owl:Class>
                <owl:unionOf rdf:parseType="Collection">
                    <rdf:Description rdf:about="http://www.ontologydesignpatterns.org/ont/is/mandlerpaganis.owl#ImageSchema"/>
                    <rdf:Description rdf:about="http://www.ontologydesignpatterns.org/ont/is/mandlerpaganis.owl#SpatialPrimitive"/>
                </owl:unionOf>
            </owl:Class>
        </rdfs:domain>
        <rdfs:range rdf:resource="http://www.ontologydesignpatterns.org/ont/is/mandlerpaganis.owl#IS_Grouping"/>
        <rdfs:comment>Some ImageSchemas or SpatialPrimitive is groupedIn some IS_Grouping following some IS_GorupingCriterion.</rdfs:comment>
    </owl:ObjectProperty>
    


    <!-- http://www.ontologydesignpatterns.org/ont/is/mandlerpaganis.owl#groups -->

    <owl:ObjectProperty rdf:about="http://www.ontologydesignpatterns.org/ont/is/mandlerpaganis.owl#groups">
        <rdfs:domain rdf:resource="http://www.ontologydesignpatterns.org/ont/is/mandlerpaganis.owl#IS_Grouping"/>
        <rdfs:range>
            <owl:Class>
                <owl:unionOf rdf:parseType="Collection">
                    <rdf:Description rdf:about="http://www.ontologydesignpatterns.org/ont/is/mandlerpaganis.owl#ImageSchema"/>
                    <rdf:Description rdf:about="http://www.ontologydesignpatterns.org/ont/is/mandlerpaganis.owl#SpatialPrimitive"/>
                </owl:unionOf>
            </owl:Class>
        </rdfs:range>
        <rdfs:comment>Some IS_Grouping groups some ImageSchema or SpatialPrimitive following some IS_GroupingCriterion.</rdfs:comment>
    </owl:ObjectProperty>
    


    <!-- http://www.ontologydesignpatterns.org/ont/is/mandlerpaganis.owl#hasSpatialInput -->

    <owl:ObjectProperty rdf:about="http://www.ontologydesignpatterns.org/ont/is/mandlerpaganis.owl#hasSpatialInput">
        <owl:inverseOf rdf:resource="http://www.ontologydesignpatterns.org/ont/is/mandlerpaganis.owl#isTopologyProviderFor"/>
        <rdfs:domain rdf:resource="http://www.ontologydesignpatterns.org/ont/is/mandlerpaganis.owl#SchematicIntegration"/>
        <rdfs:range>
            <owl:Class>
                <owl:unionOf rdf:parseType="Collection">
                    <rdf:Description rdf:about="http://www.ontologydesignpatterns.org/ont/is/mandlerpaganis.owl#ImageSchema"/>
                    <rdf:Description rdf:about="http://www.ontologydesignpatterns.org/ont/is/mandlerpaganis.owl#SpatialPrimitive"/>
                </owl:unionOf>
            </owl:Class>
        </rdfs:range>
        <rdfs:comment>&quot;This process is similar to what is called a s i m p l e x n e t w o r k in
Conceptual Integration Theory (Fauconnier &amp; Turner, 2002, pp. 121−122). In a simplex network, an unstructured element becomes blended with a structured input space. In the resulting blend, the unstructured element assumes a relevant role within the organizing frame imported from the structured input space.&quot;
(Mandler &amp; Pagán Cánovas 2014)</rdfs:comment>
    </owl:ObjectProperty>
    


    <!-- http://www.ontologydesignpatterns.org/ont/is/mandlerpaganis.owl#isTopologyProviderFor -->

    <owl:ObjectProperty rdf:about="http://www.ontologydesignpatterns.org/ont/is/mandlerpaganis.owl#isTopologyProviderFor">
        <rdfs:comment>&quot;This process is similar to what is called a s i m p l e x n e t w o r k in
Conceptual Integration Theory (Fauconnier &amp; Turner, 2002, pp. 121−122). In a simplex network, an unstructured element becomes blended with a structured input space. In the resulting blend, the unstructured element assumes a relevant role within the organizing frame imported from the structured input space.&quot;
(Mandler &amp; Pagán Cánovas 2014)</rdfs:comment>
    </owl:ObjectProperty>
    


    <!-- http://www.ontologydesignpatterns.org/ont/is/mandlerpaganis.owl#makesUseOf -->

    <owl:ObjectProperty rdf:about="http://www.ontologydesignpatterns.org/ont/is/mandlerpaganis.owl#makesUseOf">
        <owl:inverseOf rdf:resource="http://www.ontologydesignpatterns.org/ont/is/mandlerpaganis.owl#spatialPrimitiveFor"/>
        <rdfs:domain>
            <owl:Class>
                <owl:unionOf rdf:parseType="Collection">
                    <rdf:Description rdf:about="http://www.ontologydesignpatterns.org/ont/is/mandlerpaganis.owl#IS_Grouping"/>
                    <rdf:Description rdf:about="http://www.ontologydesignpatterns.org/ont/is/mandlerpaganis.owl#ImageSchema"/>
                    <rdf:Description rdf:about="http://www.ontologydesignpatterns.org/ont/is/mandlerpaganis.owl#SchematicIntegration"/>
                </owl:unionOf>
            </owl:Class>
        </rdfs:domain>
        <rdfs:range rdf:resource="http://www.ontologydesignpatterns.org/ont/is/mandlerpaganis.owl#SpatialPrimitive"/>
        <rdfs:comment>This relation is used to assert that some ImageSchema or IS_Grouping makesUseOf some SpatialPrimitive.</rdfs:comment>
    </owl:ObjectProperty>
    


    <!-- http://www.ontologydesignpatterns.org/ont/is/mandlerpaganis.owl#spatialPrimitiveFor -->

    <owl:ObjectProperty rdf:about="http://www.ontologydesignpatterns.org/ont/is/mandlerpaganis.owl#spatialPrimitiveFor">
        <rdfs:domain rdf:resource="http://www.ontologydesignpatterns.org/ont/is/mandlerpaganis.owl#SpatialPrimitive"/>
        <rdfs:range>
            <owl:Class>
                <owl:unionOf rdf:parseType="Collection">
                    <rdf:Description rdf:about="http://www.ontologydesignpatterns.org/ont/is/mandlerpaganis.owl#IS_Grouping"/>
                    <rdf:Description rdf:about="http://www.ontologydesignpatterns.org/ont/is/mandlerpaganis.owl#ImageSchema"/>
                    <rdf:Description rdf:about="http://www.ontologydesignpatterns.org/ont/is/mandlerpaganis.owl#SchematicIntegration"/>
                </owl:unionOf>
            </owl:Class>
        </rdfs:range>
        <rdfs:comment>This relation is used to assert that some SpatialPrimitive is spatialPrimitiveFor some ImageSchema.</rdfs:comment>
    </owl:ObjectProperty>
    


    <!-- 
    ///////////////////////////////////////////////////////////////////////////////////////
    //
    // Classes
    //
    ///////////////////////////////////////////////////////////////////////////////////////
     -->

    


    <!-- http://www.ontologydesignpatterns.org/ont/dul/DUL.owl#Concept -->

    <owl:Class rdf:about="http://www.ontologydesignpatterns.org/ont/dul/DUL.owl#Concept">
        <rdfs:comment>A Concept is a SocialObject, and isDefinedIn some Description; once defined, a Concept can be used in other Description(s). If a Concept isDefinedIn exactly one Description, see the LocalConcept class. The classifies relation relates Concept(s) to Entity(s) at some TimeInterval.</rdfs:comment>
    </owl:Class>
    


    <!-- http://www.ontologydesignpatterns.org/ont/is/mandlerpaganis.owl#EarlyConcept -->

    <owl:Class rdf:about="http://www.ontologydesignpatterns.org/ont/is/mandlerpaganis.owl#EarlyConcept">
        <rdfs:subClassOf rdf:resource="http://www.ontologydesignpatterns.org/ont/dul/DUL.owl#Concept"/>
        <rdfs:comment>A Concept developed in the early stages of life. In this module in the first 6 to 8 months of life.</rdfs:comment>
    </owl:Class>
    


    <!-- http://www.ontologydesignpatterns.org/ont/is/mandlerpaganis.owl#IS_Approach -->

    <owl:Class rdf:about="http://www.ontologydesignpatterns.org/ont/is/mandlerpaganis.owl#IS_Approach">
        <rdfs:comment>The approach considered to classify, conceptualize and cluster Image Schemas.</rdfs:comment>
    </owl:Class>
    


    <!-- http://www.ontologydesignpatterns.org/ont/is/mandlerpaganis.owl#IS_Combination -->

    <owl:Class rdf:about="http://www.ontologydesignpatterns.org/ont/is/mandlerpaganis.owl#IS_Combination">
        <rdfs:comment>The way in which Image Schemas or Spatial Primitives combine with each other.</rdfs:comment>
    </owl:Class>
    


    <!-- http://www.ontologydesignpatterns.org/ont/is/mandlerpaganis.owl#IS_ComplexityCriterion -->

    <owl:Class rdf:about="http://www.ontologydesignpatterns.org/ont/is/mandlerpaganis.owl#IS_ComplexityCriterion">
        <ismeta:bibRef>&quot;It is important for cognitive semantics to be aware of preverbal conceptual understanding. In particular, finding the meanings that preverbal infants ascribe to events gives us information about the most fundamental image schemas and how they differ from more complex schematic integrations.&quot;
(Mandler &amp; Pagán Cánovas 2014)</ismeta:bibRef>
    </owl:Class>
    


    <!-- http://www.ontologydesignpatterns.org/ont/is/mandlerpaganis.owl#IS_Grouping -->

    <owl:Class rdf:about="http://www.ontologydesignpatterns.org/ont/is/mandlerpaganis.owl#IS_Grouping">
        <rdfs:comment>The way in which Image Schemas are grouped together.</rdfs:comment>
    </owl:Class>
    


    <!-- http://www.ontologydesignpatterns.org/ont/is/mandlerpaganis.owl#ImageSchema -->

    <owl:Class rdf:about="http://www.ontologydesignpatterns.org/ont/is/mandlerpaganis.owl#ImageSchema">
        <ismeta:bibRef>&quot;image schemas are simple spatial stories built from Spatial Primitives&quot; 

(Mandler &amp; Pagán Cánovas 2014: 1)</ismeta:bibRef>
    </owl:Class>
    


    <!-- http://www.ontologydesignpatterns.org/ont/is/mandlerpaganis.owl#SchematicIntegration -->

    <owl:Class rdf:about="http://www.ontologydesignpatterns.org/ont/is/mandlerpaganis.owl#SchematicIntegration">
        <ismeta:bibRef>&quot;The enriched spatial concept that results from blending a spatial event with a non-spatial component.&quot;
(Mandler &amp; Pagán Cánovas 2014)</ismeta:bibRef>
        <ismeta:bibRef>&quot;The first conceptual representations to include non-spatial elements, by projecting feelings or non-spatial perceptions to blends structured by image schemas.&quot;
(Mandler &amp; Pagán Cánovas 2014)</ismeta:bibRef>
        <ismeta:bibRef>&quot;schematic integrations use the first two types (Spatial Primitives and Image Schemas) to build concepts that include non-spatial elements, such as force and emotion.
(Mandler &amp; Pagán Cánovas 2014: 1)</ismeta:bibRef>
    </owl:Class>
    


    <!-- http://www.ontologydesignpatterns.org/ont/is/mandlerpaganis.owl#SpatialPrimitive -->

    <owl:Class rdf:about="http://www.ontologydesignpatterns.org/ont/is/mandlerpaganis.owl#SpatialPrimitive">
        <ismeta:bibRef>“Spatial primitives are the first conceptual building blocks formed in infancy” 

(Mandler &amp; Pagán Cánovas 2014: 1)</ismeta:bibRef>
    </owl:Class>
    


    <!-- 
    ///////////////////////////////////////////////////////////////////////////////////////
    //
    // Individuals
    //
    ///////////////////////////////////////////////////////////////////////////////////////
     -->

    


    <!-- http://www.ontologydesignpatterns.org/ont/is/mandlerpaganis.owl#ANIMATE_MOVE -->

    <owl:NamedIndividual rdf:about="http://www.ontologydesignpatterns.org/ont/is/mandlerpaganis.owl#ANIMATE_MOVE">
        <rdf:type rdf:resource="http://www.ontologydesignpatterns.org/ont/is/mandlerpaganis.owl#SpatialPrimitive"/>
        <spatialPrimitiveFor rdf:resource="http://www.ontologydesignpatterns.org/ont/is/mandlerpaganis.owl#GOAL_PATHS"/>
        <ismeta:bibRef>Mandler, J. M., &amp; Cánovas, C. P. (2014). On defining image schemas. Language and cognition, 6(4), 510-532.</ismeta:bibRef>
    </owl:NamedIndividual>
    


    <!-- http://www.ontologydesignpatterns.org/ont/is/mandlerpaganis.owl#ANIMATE_THING -->

    <owl:NamedIndividual rdf:about="http://www.ontologydesignpatterns.org/ont/is/mandlerpaganis.owl#ANIMATE_THING">
        <rdf:type rdf:resource="http://www.ontologydesignpatterns.org/ont/is/mandlerpaganis.owl#EarlyConcept"/>
        <rdf:type rdf:resource="http://www.ontologydesignpatterns.org/ont/is/mandlerpaganis.owl#IS_Combination"/>
        <combinationResultsFrom rdf:resource="http://www.ontologydesignpatterns.org/ont/is/mandlerpaganis.owl#ANIMATE_MOVE"/>
        <combinationResultsFrom rdf:resource="http://www.ontologydesignpatterns.org/ont/is/mandlerpaganis.owl#THING"/>
        <ismeta:bibRef>Mandler, J. M., &amp; Cánovas, C. P. (2014). On defining image schemas. Language and cognition, 6(4), 510-532.</ismeta:bibRef>
    </owl:NamedIndividual>
    


    <!-- http://www.ontologydesignpatterns.org/ont/is/mandlerpaganis.owl#APPEAR -->

    <owl:NamedIndividual rdf:about="http://www.ontologydesignpatterns.org/ont/is/mandlerpaganis.owl#APPEAR">
        <rdf:type rdf:resource="http://www.ontologydesignpatterns.org/ont/is/mandlerpaganis.owl#SpatialPrimitive"/>
        <spatialPrimitiveFor rdf:resource="http://www.ontologydesignpatterns.org/ont/is/mandlerpaganis.owl#GOAL_PATHS"/>
        <spatialPrimitiveFor rdf:resource="http://www.ontologydesignpatterns.org/ont/is/mandlerpaganis.owl#OCCLUSION_AND_CONTAINMENT"/>
        <ismeta:bibRef>Mandler, J. M., &amp; Cánovas, C. P. (2014). On defining image schemas. Language and cognition, 6(4), 510-532.</ismeta:bibRef>
    </owl:NamedIndividual>
    


    <!-- http://www.ontologydesignpatterns.org/ont/is/mandlerpaganis.owl#BEHIND -->

    <owl:NamedIndividual rdf:about="http://www.ontologydesignpatterns.org/ont/is/mandlerpaganis.owl#BEHIND">
        <rdf:type rdf:resource="http://www.ontologydesignpatterns.org/ont/is/mandlerpaganis.owl#SpatialPrimitive"/>
        <spatialPrimitiveFor rdf:resource="http://www.ontologydesignpatterns.org/ont/is/mandlerpaganis.owl#GOAL_PATHS"/>
        <spatialPrimitiveFor rdf:resource="http://www.ontologydesignpatterns.org/ont/is/mandlerpaganis.owl#OCCLUSION_AND_CONTAINMENT"/>
        <ismeta:bibRef>Mandler, J. M., &amp; Cánovas, C. P. (2014). On defining image schemas. Language and cognition, 6(4), 510-532.</ismeta:bibRef>
    </owl:NamedIndividual>
    


    <!-- http://www.ontologydesignpatterns.org/ont/is/mandlerpaganis.owl#BLOCKED_MOVE -->

    <owl:NamedIndividual rdf:about="http://www.ontologydesignpatterns.org/ont/is/mandlerpaganis.owl#BLOCKED_MOVE">
        <rdf:type rdf:resource="http://www.ontologydesignpatterns.org/ont/is/mandlerpaganis.owl#SpatialPrimitive"/>
        <spatialPrimitiveFor rdf:resource="http://www.ontologydesignpatterns.org/ont/is/mandlerpaganis.owl#GOAL_PATHS"/>
        <ismeta:bibRef>Mandler, J. M., &amp; Cánovas, C. P. (2014). On defining image schemas. Language and cognition, 6(4), 510-532.</ismeta:bibRef>
    </owl:NamedIndividual>
    


    <!-- http://www.ontologydesignpatterns.org/ont/is/mandlerpaganis.owl#CONTACT -->

    <owl:NamedIndividual rdf:about="http://www.ontologydesignpatterns.org/ont/is/mandlerpaganis.owl#CONTACT">
        <rdf:type rdf:resource="http://www.ontologydesignpatterns.org/ont/is/mandlerpaganis.owl#SpatialPrimitive"/>
        <ismeta:bibRef>Mandler, J. M., &amp; Cánovas, C. P. (2014). On defining image schemas. Language and cognition, 6(4), 510-532.</ismeta:bibRef>
    </owl:NamedIndividual>
    


    <!-- http://www.ontologydesignpatterns.org/ont/is/mandlerpaganis.owl#CONTAINER -->

    <owl:NamedIndividual rdf:about="http://www.ontologydesignpatterns.org/ont/is/mandlerpaganis.owl#CONTAINER">
        <rdf:type rdf:resource="http://www.ontologydesignpatterns.org/ont/is/mandlerpaganis.owl#SpatialPrimitive"/>
        <spatialPrimitiveFor rdf:resource="http://www.ontologydesignpatterns.org/ont/is/mandlerpaganis.owl#OCCLUSION_AND_CONTAINMENT"/>
        <ismeta:bibRef>Mandler, J. M., &amp; Cánovas, C. P. (2014). On defining image schemas. Language and cognition, 6(4), 510-532.</ismeta:bibRef>
    </owl:NamedIndividual>
    


    <!-- http://www.ontologydesignpatterns.org/ont/is/mandlerpaganis.owl#DISAPPEAR -->

    <owl:NamedIndividual rdf:about="http://www.ontologydesignpatterns.org/ont/is/mandlerpaganis.owl#DISAPPEAR">
        <rdf:type rdf:resource="http://www.ontologydesignpatterns.org/ont/is/mandlerpaganis.owl#SpatialPrimitive"/>
        <spatialPrimitiveFor rdf:resource="http://www.ontologydesignpatterns.org/ont/is/mandlerpaganis.owl#GOAL_PATHS"/>
        <spatialPrimitiveFor rdf:resource="http://www.ontologydesignpatterns.org/ont/is/mandlerpaganis.owl#OCCLUSION_AND_CONTAINMENT"/>
        <ismeta:bibRef>Mandler, J. M., &amp; Cánovas, C. P. (2014). On defining image schemas. Language and cognition, 6(4), 510-532.</ismeta:bibRef>
    </owl:NamedIndividual>
    


    <!-- http://www.ontologydesignpatterns.org/ont/is/mandlerpaganis.owl#DevelopmentalPerspective -->

    <owl:NamedIndividual rdf:about="http://www.ontologydesignpatterns.org/ont/is/mandlerpaganis.owl#DevelopmentalPerspective">
        <rdf:type rdf:resource="http://www.ontologydesignpatterns.org/ont/is/mandlerpaganis.owl#IS_Approach"/>
        <rdfs:comment>Developmental perspective in terms of simple early spatial dimensions (e.g. ANIMACY, INANIMACY, AGENCY, CONTAINMENT) that quickly develop into more complex structures, combining with other concepts.</rdfs:comment>
    </owl:NamedIndividual>
    


    <!-- http://www.ontologydesignpatterns.org/ont/is/mandlerpaganis.owl#EMOTION -->

    <owl:NamedIndividual rdf:about="http://www.ontologydesignpatterns.org/ont/is/mandlerpaganis.owl#EMOTION">
        <rdf:type rdf:resource="http://www.ontologydesignpatterns.org/ont/is/mandlerpaganis.owl#SchematicIntegration"/>
        <ismeta:bibRef>Mandler, J. M., &amp; Cánovas, C. P. (2014). On defining image schemas. Language and cognition, 6(4), 510-532.</ismeta:bibRef>
    </owl:NamedIndividual>
    


    <!-- http://www.ontologydesignpatterns.org/ont/is/mandlerpaganis.owl#END_PATH -->

    <owl:NamedIndividual rdf:about="http://www.ontologydesignpatterns.org/ont/is/mandlerpaganis.owl#END_PATH">
        <rdf:type rdf:resource="http://www.ontologydesignpatterns.org/ont/is/mandlerpaganis.owl#SpatialPrimitive"/>
        <spatialPrimitiveFor rdf:resource="http://www.ontologydesignpatterns.org/ont/is/mandlerpaganis.owl#GOAL_PATHS"/>
        <ismeta:bibRef>Mandler, J. M., &amp; Cánovas, C. P. (2014). On defining image schemas. Language and cognition, 6(4), 510-532.</ismeta:bibRef>
    </owl:NamedIndividual>
    


    <!-- http://www.ontologydesignpatterns.org/ont/is/mandlerpaganis.owl#EYES -->

    <owl:NamedIndividual rdf:about="http://www.ontologydesignpatterns.org/ont/is/mandlerpaganis.owl#EYES">
        <rdf:type rdf:resource="http://www.ontologydesignpatterns.org/ont/is/mandlerpaganis.owl#SpatialPrimitive"/>
        <ismeta:bibRef>Mandler, J. M., &amp; Cánovas, C. P. (2014). On defining image schemas. Language and cognition, 6(4), 510-532.</ismeta:bibRef>
    </owl:NamedIndividual>
    


    <!-- http://www.ontologydesignpatterns.org/ont/is/mandlerpaganis.owl#FORCE -->

    <owl:NamedIndividual rdf:about="http://www.ontologydesignpatterns.org/ont/is/mandlerpaganis.owl#FORCE">
        <rdf:type rdf:resource="http://www.ontologydesignpatterns.org/ont/is/mandlerpaganis.owl#SchematicIntegration"/>
        <hasSpatialInput rdf:resource="http://www.ontologydesignpatterns.org/ont/is/mandlerpaganis.owl#BLOCKED_MOVE"/>
        <ismeta:bibRef>Mandler, J. M., &amp; Cánovas, C. P. (2014). On defining image schemas. Language and cognition, 6(4), 510-532.</ismeta:bibRef>
    </owl:NamedIndividual>
    


    <!-- http://www.ontologydesignpatterns.org/ont/is/mandlerpaganis.owl#GOAL_PATHS -->

    <owl:NamedIndividual rdf:about="http://www.ontologydesignpatterns.org/ont/is/mandlerpaganis.owl#GOAL_PATHS">
        <rdf:type rdf:resource="http://www.ontologydesignpatterns.org/ont/is/mandlerpaganis.owl#IS_Grouping"/>
        <groups rdf:resource="http://www.ontologydesignpatterns.org/ont/is/mandlerpaganis.owl#PATH_TO_THING"/>
        <ismeta:bibRef>Mandler, J. M., &amp; Cánovas, C. P. (2014). On defining image schemas. Language and cognition, 6(4), 510-532.</ismeta:bibRef>
    </owl:NamedIndividual>
    


    <!-- http://www.ontologydesignpatterns.org/ont/is/mandlerpaganis.owl#INTO -->

    <owl:NamedIndividual rdf:about="http://www.ontologydesignpatterns.org/ont/is/mandlerpaganis.owl#INTO">
        <rdf:type rdf:resource="http://www.ontologydesignpatterns.org/ont/is/mandlerpaganis.owl#SpatialPrimitive"/>
        <spatialPrimitiveFor rdf:resource="http://www.ontologydesignpatterns.org/ont/is/mandlerpaganis.owl#GOAL_PATHS"/>
        <spatialPrimitiveFor rdf:resource="http://www.ontologydesignpatterns.org/ont/is/mandlerpaganis.owl#OCCLUSION_AND_CONTAINMENT"/>
        <ismeta:bibRef>Mandler, J. M., &amp; Cánovas, C. P. (2014). On defining image schemas. Language and cognition, 6(4), 510-532.</ismeta:bibRef>
    </owl:NamedIndividual>
    


    <!-- http://www.ontologydesignpatterns.org/ont/is/mandlerpaganis.owl#LINK -->

    <owl:NamedIndividual rdf:about="http://www.ontologydesignpatterns.org/ont/is/mandlerpaganis.owl#LINK">
        <rdf:type rdf:resource="http://www.ontologydesignpatterns.org/ont/is/mandlerpaganis.owl#SpatialPrimitive"/>
        <spatialPrimitiveFor rdf:resource="http://www.ontologydesignpatterns.org/ont/is/mandlerpaganis.owl#GOAL_PATHS"/>
        <spatialPrimitiveFor rdf:resource="http://www.ontologydesignpatterns.org/ont/is/mandlerpaganis.owl#OCCLUSION_AND_CONTAINMENT"/>
        <ismeta:bibRef>Mandler, J. M., &amp; Cánovas, C. P. (2014). On defining image schemas. Language and cognition, 6(4), 510-532.</ismeta:bibRef>
    </owl:NamedIndividual>
    


    <!-- http://www.ontologydesignpatterns.org/ont/is/mandlerpaganis.owl#LOCATION -->

    <owl:NamedIndividual rdf:about="http://www.ontologydesignpatterns.org/ont/is/mandlerpaganis.owl#LOCATION">
        <rdf:type rdf:resource="http://www.ontologydesignpatterns.org/ont/is/mandlerpaganis.owl#SpatialPrimitive"/>
        <spatialPrimitiveFor rdf:resource="http://www.ontologydesignpatterns.org/ont/is/mandlerpaganis.owl#GOAL_PATHS"/>
        <ismeta:bibRef>Mandler, J. M., &amp; Cánovas, C. P. (2014). On defining image schemas. Language and cognition, 6(4), 510-532.</ismeta:bibRef>
    </owl:NamedIndividual>
    


    <!-- http://www.ontologydesignpatterns.org/ont/is/mandlerpaganis.owl#MOVE -->

    <owl:NamedIndividual rdf:about="http://www.ontologydesignpatterns.org/ont/is/mandlerpaganis.owl#MOVE">
        <rdf:type rdf:resource="http://www.ontologydesignpatterns.org/ont/is/mandlerpaganis.owl#SpatialPrimitive"/>
        <spatialPrimitiveFor rdf:resource="http://www.ontologydesignpatterns.org/ont/is/mandlerpaganis.owl#GOAL_PATHS"/>
        <ismeta:bibRef>Mandler, J. M., &amp; Cánovas, C. P. (2014). On defining image schemas. Language and cognition, 6(4), 510-532.</ismeta:bibRef>
    </owl:NamedIndividual>
    


    <!-- http://www.ontologydesignpatterns.org/ont/is/mandlerpaganis.owl#OCCLUSION_AND_CONTAINMENT -->

    <owl:NamedIndividual rdf:about="http://www.ontologydesignpatterns.org/ont/is/mandlerpaganis.owl#OCCLUSION_AND_CONTAINMENT">
        <rdf:type rdf:resource="http://www.ontologydesignpatterns.org/ont/is/mandlerpaganis.owl#IS_Grouping"/>
        <groups rdf:resource="http://www.ontologydesignpatterns.org/ont/is/mandlerpaganis.owl#THING_INTO_CONTAINER"/>
        <ismeta:bibRef>Mandler, J. M., &amp; Cánovas, C. P. (2014). On defining image schemas. Language and cognition, 6(4), 510-532.</ismeta:bibRef>
    </owl:NamedIndividual>
    


    <!-- http://www.ontologydesignpatterns.org/ont/is/mandlerpaganis.owl#OPEN -->

    <owl:NamedIndividual rdf:about="http://www.ontologydesignpatterns.org/ont/is/mandlerpaganis.owl#OPEN">
        <rdf:type rdf:resource="http://www.ontologydesignpatterns.org/ont/is/mandlerpaganis.owl#SpatialPrimitive"/>
        <spatialPrimitiveFor rdf:resource="http://www.ontologydesignpatterns.org/ont/is/mandlerpaganis.owl#OCCLUSION_AND_CONTAINMENT"/>
        <ismeta:bibRef>Mandler, J. M., &amp; Cánovas, C. P. (2014). On defining image schemas. Language and cognition, 6(4), 510-532.</ismeta:bibRef>
    </owl:NamedIndividual>
    


    <!-- http://www.ontologydesignpatterns.org/ont/is/mandlerpaganis.owl#OUT_OF -->

    <owl:NamedIndividual rdf:about="http://www.ontologydesignpatterns.org/ont/is/mandlerpaganis.owl#OUT_OF">
        <rdf:type rdf:resource="http://www.ontologydesignpatterns.org/ont/is/mandlerpaganis.owl#SpatialPrimitive"/>
        <spatialPrimitiveFor rdf:resource="http://www.ontologydesignpatterns.org/ont/is/mandlerpaganis.owl#GOAL_PATHS"/>
        <spatialPrimitiveFor rdf:resource="http://www.ontologydesignpatterns.org/ont/is/mandlerpaganis.owl#OCCLUSION_AND_CONTAINMENT"/>
        <ismeta:bibRef>Mandler, J. M., &amp; Cánovas, C. P. (2014). On defining image schemas. Language and cognition, 6(4), 510-532.</ismeta:bibRef>
    </owl:NamedIndividual>
    


    <!-- http://www.ontologydesignpatterns.org/ont/is/mandlerpaganis.owl#PATH -->

    <owl:NamedIndividual rdf:about="http://www.ontologydesignpatterns.org/ont/is/mandlerpaganis.owl#PATH">
        <rdf:type rdf:resource="http://www.ontologydesignpatterns.org/ont/is/mandlerpaganis.owl#SpatialPrimitive"/>
        <spatialPrimitiveFor rdf:resource="http://www.ontologydesignpatterns.org/ont/is/mandlerpaganis.owl#GOAL_PATHS"/>
        <ismeta:bibRef>Mandler, J. M., &amp; Cánovas, C. P. (2014). On defining image schemas. Language and cognition, 6(4), 510-532.</ismeta:bibRef>
    </owl:NamedIndividual>
    


    <!-- http://www.ontologydesignpatterns.org/ont/is/mandlerpaganis.owl#PATH_TO -->

    <owl:NamedIndividual rdf:about="http://www.ontologydesignpatterns.org/ont/is/mandlerpaganis.owl#PATH_TO">
        <rdf:type rdf:resource="http://www.ontologydesignpatterns.org/ont/is/mandlerpaganis.owl#SpatialPrimitive"/>
        <spatialPrimitiveFor rdf:resource="http://www.ontologydesignpatterns.org/ont/is/mandlerpaganis.owl#GOAL_PATHS"/>
        <ismeta:bibRef>Mandler, J. M., &amp; Cánovas, C. P. (2014). On defining image schemas. Language and cognition, 6(4), 510-532.</ismeta:bibRef>
    </owl:NamedIndividual>
    


    <!-- http://www.ontologydesignpatterns.org/ont/is/mandlerpaganis.owl#PATH_TO_THING -->

    <owl:NamedIndividual rdf:about="http://www.ontologydesignpatterns.org/ont/is/mandlerpaganis.owl#PATH_TO_THING">
        <rdf:type rdf:resource="http://www.ontologydesignpatterns.org/ont/is/mandlerpaganis.owl#ImageSchema"/>
        <ismeta:bibRef>Mandler, J. M., &amp; Cánovas, C. P. (2014). On defining image schemas. Language and cognition, 6(4), 510-532.</ismeta:bibRef>
    </owl:NamedIndividual>
    


    <!-- http://www.ontologydesignpatterns.org/ont/is/mandlerpaganis.owl#PreverbalConceptualUnderstanding -->

    <owl:NamedIndividual rdf:about="http://www.ontologydesignpatterns.org/ont/is/mandlerpaganis.owl#PreverbalConceptualUnderstanding">
        <rdf:type rdf:resource="http://www.ontologydesignpatterns.org/ont/is/mandlerpaganis.owl#IS_ComplexityCriterion"/>
        <rdfs:comment>All the instances of ImageSchema, SpatialPrimitive and SchematicIntegration classes are taken from the same paper, namely (Mandler &amp; Pagán Cánovas 2014). All the results are based on experiments on infants from 6 to 7 months of life, so the criterion of complexity taken in consideration in this theory is the following: the first Image Schemas developed in early stage of life (6 to 8 months of life).</rdfs:comment>
    </owl:NamedIndividual>
    


    <!-- http://www.ontologydesignpatterns.org/ont/is/mandlerpaganis.owl#START_PATH -->

    <owl:NamedIndividual rdf:about="http://www.ontologydesignpatterns.org/ont/is/mandlerpaganis.owl#START_PATH">
        <rdf:type rdf:resource="http://www.ontologydesignpatterns.org/ont/is/mandlerpaganis.owl#SpatialPrimitive"/>
        <spatialPrimitiveFor rdf:resource="http://www.ontologydesignpatterns.org/ont/is/mandlerpaganis.owl#GOAL_PATHS"/>
        <ismeta:bibRef>Mandler, J. M., &amp; Cánovas, C. P. (2014). On defining image schemas. Language and cognition, 6(4), 510-532.</ismeta:bibRef>
    </owl:NamedIndividual>
    


    <!-- http://www.ontologydesignpatterns.org/ont/is/mandlerpaganis.owl#THING -->

    <owl:NamedIndividual rdf:about="http://www.ontologydesignpatterns.org/ont/is/mandlerpaganis.owl#THING">
        <rdf:type rdf:resource="http://www.ontologydesignpatterns.org/ont/is/mandlerpaganis.owl#SpatialPrimitive"/>
        <spatialPrimitiveFor rdf:resource="http://www.ontologydesignpatterns.org/ont/is/mandlerpaganis.owl#GOAL_PATHS"/>
        <spatialPrimitiveFor rdf:resource="http://www.ontologydesignpatterns.org/ont/is/mandlerpaganis.owl#OCCLUSION_AND_CONTAINMENT"/>
        <ismeta:bibRef>Mandler, J. M., &amp; Cánovas, C. P. (2014). On defining image schemas. Language and cognition, 6(4), 510-532.</ismeta:bibRef>
    </owl:NamedIndividual>
    


    <!-- http://www.ontologydesignpatterns.org/ont/is/mandlerpaganis.owl#THING_INTO_CONTAINER -->

    <owl:NamedIndividual rdf:about="http://www.ontologydesignpatterns.org/ont/is/mandlerpaganis.owl#THING_INTO_CONTAINER">
        <rdf:type rdf:resource="http://www.ontologydesignpatterns.org/ont/is/mandlerpaganis.owl#ImageSchema"/>
        <ismeta:bibRef>Mandler, J. M., &amp; Cánovas, C. P. (2014). On defining image schemas. Language and cognition, 6(4), 510-532.</ismeta:bibRef>
    </owl:NamedIndividual>
</rdf:RDF>



<!-- Generated by the OWL API (version 4.5.9.2019-02-01T07:24:44Z) https://github.com/owlcs/owlapi -->

